## introduction




$$
F_n = F_{n-1} + F_{n-2}, N>=2
$$ {\tag{1}



$$
\left(\begin{matrix} F_n\\ F_{n-1}  \end{matrix} \right) =  \left(\begin{matrix} 1 & 1 \\ 0 & 1 \end{matrix} \right)  \left(\begin{matrix} F_{n-1}\\ F_{n-2}  \end{matrix} \right) , n>=3
$$


Let:
$$
fn=\left(\begin{matrix} F_n\\ F_{n-1}  \end{matrix} \right), A=\left(\begin{matrix} 1 & 1 \\ 0 & 1 \end{matrix} \right)
$$

$$
fn=AF_{n-1}, n>=3
$$ {\tag{3}

$$
f_1 = \left(\begin{matrix}1 \\ 1  \end{matrix} \right)
$$



$$
f_n = A^{n-2}f_1
$$










## Links

